clean up

theories/syntax.sig
@@ -1,0 +1,17 @@
+action : Type
+value : Type
+gType : Type
+endpoint : Type
+dir : Type
+list : Functor
+ch : Type
+
+GEnd : gType
+GRec : (gType -> gType) -> gType
+GMsg : action -> value -> gType -> gType
+GBranch : action -> "list" (gType) -> gType
+
+EEnd : endpoint
+ERec : (endpoint -> endpoint) -> endpoint
+EMsg : dir -> ch -> value -> endpoint ->  endpoint
+EBranch : dir -> ch -> "list" (endpoint) -> endpoint
