theories/Substitutions.v
@@ -1,0 +1,144 @@
+From mathcomp Require Import all_ssreflect zify finmap.
+Require Import Paco.paco.
+Set Implicit Arguments.
+Unset Strict Implicit.
+Unset Printing Implicit Defensive.
+From Dep Require Import NewSyntax  Utils.
+
+
+Lemma injective_shift : injective S.
+Proof. intro. intros. inversion H.  done. Qed.
+
+Hint Resolve injective_shift.
+
+
+
+
+Lemma inject2 : forall sigma, injective sigma ->  injective (0 .: sigma >> succn).
+Proof. 
+intros. intro. intros. destruct x1;destruct x2;try done. inversion H0. f_equal. apply/H. done. 
+Qed.
+
+Lemma inject_comp : forall (A B C : Type) (sigma : A -> B) (sigma' : B -> C) , injective sigma -> injective sigma' -> injective (sigma >> sigma').  
+Proof. 
+intros. rewrite /funcomp. intro. intros. apply H. apply H0. done.
+Qed.
+
+
+Hint Resolve inject2.
+
+Lemma guarded_ren : forall g sigma i , (forall n, sigma n != i) -> guarded i g -> guarded i g ⟨g sigma⟩.
+Proof.
+elim;rewrite /=;simpl;intros;try done.
+asimpl. apply : H. intros. destruct n.  done. simpl. specialize H0 with n. rewrite /funcomp. lia.
+done. 
+Qed.
+
+Lemma guarded_shift1 : forall g i sigma, injective sigma ->  guarded i g -> guarded (sigma i) g ⟨g sigma⟩.
+Proof.
+elim;rewrite /=;simpl;intros;try done.
+apply/eqP. move=> HH. apply H in HH. lia. 
+asimpl. 
+have : (sigma i).+1 = ((0 .: sigma >> succn) i.+1).
+destruct i.  simpl. rewrite /funcomp. done. simpl. rewrite /funcomp. done.
+move=>->. apply H. intro. intros. destruct x1;destruct x2;try done. inversion H2. f_equal.  apply/H0. done. 
+done. 
+Qed.
+
+
+
+Lemma guarded_shift2 : forall g i sigma, injective sigma ->  guarded (sigma i) g ⟨g sigma⟩ ->  guarded i g.
+Proof.
+elim;rewrite /=;simpl;intros;try done.
+apply/eqP. move=> HH. apply (negP H0). apply/eqP. f_equal. done. 
+apply :H.  2 : { apply : H1.  } 
+asimpl. auto. 
+Qed.
+
+
+Lemma guarded_shift : forall g sigma i , injective sigma  -> guarded i g <-> guarded (sigma i) g ⟨g sigma⟩.
+
+intros. split;intros; eauto using guarded_shift1, guarded_shift2.
+Qed.
+
+
+Lemma contractive2_ren : forall g sigma, injective sigma -> (forall n, n <= sigma n) ->  contractive2  g -> contractive2 g ⟨g sigma ⟩.
+Proof.
+elim;intros;simpl;try done. 
+asimpl. split_and. have : 0 = ( 0 .: sigma >> succn) 0. done. intros. rewrite {1}x.
+
+rewrite -guarded_shift. simpl in H2. split_and. auto.
+apply H. auto.  case. done. done.  simpl in H2. split_and. apply H.  done. done. done.
+rewrite all_map. apply/allP. intro. intros. simpl. apply H. done.  done. done.  simpl in H2. apply (allP H2). done.
+Qed.
+
+
+
+Lemma guarded_sig2_ren : forall g sigma sigma' i, guarded i g ⟨g sigma⟩ -> (forall n, (sigma n) != i ->  (sigma' n) != i) -> guarded i g ⟨g sigma'⟩.
+Proof.
+elim;rewrite /=;intros;try done.
+apply H0. done.
+asimpl. apply : H. eauto. move => n.  asimpl. simpl. intros. destruct n. done. simpl in *. 
+move : H. rewrite /funcomp. intros. suff :  sigma' n != i.  lia. apply : H1. lia. 
+Qed.
+
+Lemma guarded_sig2 : forall g sigma sigma' i, guarded i g [g sigma] -> (forall n, guarded i (sigma n) -> guarded i (sigma' n)) -> guarded i g [g sigma'].
+Proof.
+elim;rewrite /=;intros;try done.
+apply H0. done.
+asimpl. apply : H. eauto. move => n.  asimpl. simpl. intros. destruct n. done. simpl in *.
+move : H. rewrite /funcomp. specialize H1 with n. move : H0. asimpl.
+intros. rewrite -guarded_shift. move : H. rewrite -guarded_shift.  move/H1. done. 
+done. done. 
+Qed.
+
+
+Lemma guarded_fv : forall g v, v \notin gType_fv g -> guarded v g.
+Proof.
+elim;rewrite /=;try done;intros.
+rewrite !inE in H. lia.
+apply H. move : H0. move/imfsetP=>HH. apply/negP=>HH'. apply HH. simpl. exists v.+1;try done.  
+rewrite !inE. split_and.
+Qed.
+
+Lemma inotin : forall g i sigma, (forall n, i !=  sigma n) -> i \notin gType_fv g ⟨g sigma ⟩.
+Proof.
+elim;rewrite /=;try done;intros. rewrite !inE. specialize H with n. lia.
+apply/imfsetP=>/=H'. destruct H'. rewrite !inE in H1.  destruct (andP H1). move : H3. asimpl. intros. apply/negP. apply : H. 2 : { apply : H3. } case. simpl. done. simpl. intros. asimpl. destruct x.  done. suff : x != sigma n. lia. 
+specialize H0 with n.  simpl in H2. subst. done. 
+rewrite !big_map big_exists. apply/negP. move/hasP=>HH. destruct HH. apply/negP. apply : H. eauto.
+2 : {  apply : H2. } auto.
+Qed.
+
+Lemma contractive2_subst : forall g sigma,contractive2 g -> (forall n, contractive2 (sigma n)) -> contractive2 g [g sigma].
+Proof. 
+elim;rewrite /=;intros;try done. 
+asimpl. split_and. 
+apply/guarded_sig2.
+instantiate (1 := (var 0 .: var >>  ⟨g ↑ ⟩)).  asimpl. done.
+case. done. simpl. intros. apply/guarded_fv. asimpl. apply/inotin. done.
+apply H. done.  intros. destruct n.  done. simpl. asimpl.  apply/contractive2_ren. done. done. done.
+apply H. done.  intros. done. 
+rewrite all_map. apply/allP. intro. intros. simpl. apply H. done. apply (allP H0). done. done.
+Qed.
+
+
+
+Lemma mu_height_ren : forall g sigma, mu_height g ⟨g sigma ⟩  = mu_height g.
+Proof.
+elim;rewrite /=;try done;intros.
+f_equal. apply : H. 
+Qed.
+
+
+
+Lemma mu_height_subst : forall g0 sigma i,  guarded  i g0 -> (forall n, n != i -> mu_height (sigma n) = 0) -> contractive2 g0 -> mu_height (g0[g sigma]) = mu_height g0.
+Proof. 
+elim; try solve [by rewrite /=];intros.
+- asimpl. simpl in H. rewrite H0. done. apply : H. 
+simpl. f_equal. asimpl. apply H with (i:=i.+1). 2 : { intros. destruct n. simpl. done. simpl. asimpl.
+rewrite mu_height_ren. apply H1. lia.  } intros. apply : H0. eauto. simpl in H2. split_and.
+Qed. 
+
+
+
